lean/NesyLink.lean
@@ -1,17 +1,5 @@
-/-
-  Environment.lean        类型、单步转移等等
-  Strategy.lean           多步执行、BFS、策略性质证明
-  TaskInitStates_1.lean   任务 1 初态
-  TaskInitStates_2.lean   任务 2 初态
-  TaskInitStates_3.lean   任务 3 初态
-  TaskInitStates_4.lean   任务 4 初态
-  TaskInitStates_5.lean   任务 5 初态
--/
-
-import NesyLink.Environment
+import NesyLink.Env1
+import NesyLink.Env2
 import NesyLink.Strategy
-import NesyLink.TaskInitStates_1
-import NesyLink.TaskInitStates_2
-import NesyLink.TaskInitStates_3
-import NesyLink.TaskInitStates_4
-import NesyLink.TaskInitStates_5
+import NesyLink.StrategySafety
+import NesyLink.Axioms
