lean/NesyLink/Env1.lean
@@ -1,0 +1,78 @@
+def Coord := Fin 8 × Fin 10
+deriving instance DecidableEq for Coord
+
+inductive Direction where
+  | up
+  | down
+  | left
+  | right
+  deriving DecidableEq, Repr, Inhabited
+
+inductive Item where
+  | key
+  | sword
+  deriving DecidableEq, Repr
+
+--===================
+inductive Action where
+  | wait
+  | move
+  | buttonA
+  | buttonB
+  deriving DecidableEq, Repr
+
+structure Input where
+ direction : Direction
+ action : Action
+ deriving Repr
+
+inductive Condition where
+  | None
+  | consumeKey
+  | ButtonPressed (buttonPos : Coord)
+  | EnimyCleared
+  deriving DecidableEq
+
+inductive Tile where
+  | ground
+  | wall
+  | spike
+  | button (pressed : Bool)
+  | switch (state : Nat)
+  | chest (opened : Bool) (content : Item) (hidden : Bool) (cond : Condition)
+  | bridge (switchRoom : Nat) (switchCoord : Coord) (activeState : Nat)
+  | door (id : Nat)
+  deriving DecidableEq
+
+structure DoorInfo where
+  id : Nat
+  condition : Condition
+  isOpened : Bool
+  orientation : Direction
+  targetRoom : Nat
+  targetCoord : Coord
+
+structure Enemy where
+  hp : Nat
+  coord : Coord
+
+structure Room where
+  spawn : Coord
+  layout : List (List Tile)
+  doors : List DoorInfo
+  enemies : List Enemy
+  inv_height : layout.length = 8
+  inv_width  : ∀ row ∈ layout, row.length = 10
+
+structure Player where
+  room : Nat
+  coord : Coord
+  health : Nat
+  gold : Nat
+  key : Nat
+  hasSword : Bool
+
+structure GameState where
+  round : Nat
+  player : Player
+  rooms : Nat → Room
