lean/lakefile.lean
@@ -2,7 +2,7 @@ import Lake
 open Lake DSL
 
 package «nesylink-lean» where
-  leanVersion := "v4.29.0-rc6"
+  
 
 @[default_target]
 lean_lib NesyLink where
